use the generated rel for the serializer'

src/cddl/pulse/CDDL.Pulse.Serialize.Base.fst
@@ -45,6 +45,46 @@ let impl_serialize
       pure (impl_serialize_post s v w res)
     )
 
+noextract [@@noextract_to "krml"]
+let coerce_spec
+  (#t: typ)
+  (#tgt: Type0)
+  (#inj: bool)
+  (ps: spec t tgt inj)
+  (tgt' : Type0)
+  (sq: squash (tgt == tgt'))
+: Tot (spec t tgt' inj)
+= ps
+
+inline_for_extraction noextract [@@noextract_to "krml"]
+fn impl_serialize_cast_rel
+    (#[@@@erasable] t: Ghost.erased typ)
+    (#tgt: Type0)
+    (#[@@@erasable] inj: Ghost.erased bool)
+    (#[@@@erasable] ps: Ghost.erased (spec t tgt inj))
+    (#impl_tgt: Type0)
+    (#r: rel impl_tgt tgt)
+    (i: impl_serialize ps r)
+    (#tgt': Type0)
+    (#impl_tgt': Type0)
+    (r': rel impl_tgt' tgt')
+    (sq1: squash (tgt == tgt'))
+    (sq2: squash (impl_tgt == impl_tgt'))
+    (sq3: squash (r' == r))
+: impl_serialize #(Ghost.reveal t) #tgt' #(Ghost.reveal inj) (coerce_spec (Ghost.reveal ps) tgt' sq1) #impl_tgt' r'
+= 
+  (c: _)
+  (#v: _)
+  (out: _)
+{
+  Trade.rewrite_with_trade
+    (r' c v)
+    (r c v); 
+  let res = i c out;
+  Trade.elim _ _;
+  res
+}
+
 let impl_serialize_t_eq
     (#t: typ)
     (#tgt: Type0)
